wip

Matroid/Constructions/ImagePreimage.lean
@@ -6,148 +6,155 @@ open Set Function
 variable {α β : Type _} {f : α → β} {E I s : Set α}
 
 namespace Matroid
-  
-/-- The pullback of a matroid on `β` by a function `f : α → β` to a matroid on `α`. Elements with 
-  the same image are parallel. -/
-def preimage (M : Matroid β) (E : Set α) (f : α → β) : Matroid α := matroid_of_indep
-  E ( fun I ↦ M.Indep (f '' I) ∧ InjOn f I ∧ I ⊆ E ) ( by simp )
-  ( fun I J ⟨h, h', hE⟩ hIJ ↦ ⟨h.subset (image_subset _ hIJ), InjOn.mono hIJ h', hIJ.trans hE⟩ )
+
+/-- The pullback of a matroid on `β` by a function `f : α → β` to a matroid on `α`.
+  Elements with the same image are parallel and the ground set is `f ⁻¹' M.E`. -/
+def preimage (M : Matroid β) (f : α → β) : Matroid α := matroid_of_indep
+  (f ⁻¹' M.E) (fun I ↦ M.Indep (f '' I) ∧ InjOn f I) ( by simp )
+  ( fun I J ⟨h, h'⟩ hIJ ↦ ⟨h.subset (image_subset _ hIJ), InjOn.mono hIJ h'⟩ )
   ( by
-    rintro I J ⟨hI, hIinj, hIE⟩ hImax hJmax
+    rintro I B ⟨hI, hIinj⟩ hImax hBmax
+    simp only [mem_maximals_iff, mem_setOf_eq, hI, hIinj, and_self, and_imp,
+      true_and, not_forall, exists_prop, exists_and_left] at hImax hBmax
 
-    simp only [mem_maximals_iff, mem_setOf_eq, and_imp, hI, hIinj, hIE, and_self, true_and, 
-      not_forall, exists_prop, exists_and_left] at hJmax hImax 
-    
-    obtain ⟨B', hB', hB'inj, hB'E, hIB', hne⟩ := hImax 
-    obtain ⟨⟨hJ, hJinj, hJE⟩, hJmax⟩ := hJmax
-  
-    have hi : (M ↾ f '' E).Indep (f '' I) := hI.indep_restrict_of_subset (image_subset f hIE)
+    obtain ⟨I', hI', hI'inj, hII', hne⟩ := hImax
 
-    have h1 : ¬(M ↾ f '' E).Base (f '' I)
-    · exact fun hB ↦ hne <| (hB'inj.image_eq_image_iff_of_subset hIB' Subset.rfl).1
-        (hB.eq_of_subset_indep (hB'.indep_restrict_of_subset (image_subset _ hB'E))
-        (image_subset _ hIB'))
-      
-    have h2 : (M ↾ f '' E).Base (f '' J)
-    · apply (hJ.indep_restrict_of_subset (image_subset _ hJE)).base_of_maximal
-      simp_rw [restrict_indep_iff]
-      rintro K' ⟨hK', hK'E⟩ hJK'
-      obtain ⟨K, hJK, hKE, hKinj, rfl⟩ := hJinj.exists_injOn_superset_image hJE hJK' hK'E
-      rw [hJmax hK' hKinj hKE]
-      rwa [←hKinj.image_subset_image_iff_of_subset hJK Subset.rfl]
-    
-    obtain ⟨_, ⟨⟨e, heJ, rfl⟩, heI⟩, hi⟩ := hi.exists_insert_of_not_base h1 h2
-    have heI' : e ∉ I := fun heI' ↦ heI (mem_image_of_mem f heI')
-    refine' ⟨e, ⟨heJ, heI'⟩, _, _, insert_subset (hJE heJ) hIE⟩ 
-    · rw [image_insert_eq]
-      exact hi.of_restrict
-    rwa [injOn_insert heI', and_iff_right hIinj] )
+    have h₁ : ¬(M ↾ range f).Base (f '' I)
+    · refine fun hB ↦ hne ?_
+      have h_im := hB.eq_of_subset_indep (by simpa) (image_subset _ hII')
+      rwa [hI'inj.image_eq_image_iff_of_subset hII' Subset.rfl] at h_im
+
+    have h₂ : (M ↾ range f).Base (f '' B)
+    · refine Indep.base_of_maximal (by simpa using hBmax.1.1) (fun J hJi hBJ ↦ ?_)
+      simp only [restrict_indep_iff] at hJi
+      obtain ⟨J₀, hBJ₀, hJ₀⟩ := hBmax.1.2.bijOn_image.extend hBJ hJi.2
+      obtain rfl := hJ₀.image_eq
+      rw [hBmax.2 hJi.1 hJ₀.injOn hBJ₀]
+
+    obtain ⟨_, ⟨⟨e, he, rfl⟩, he'⟩, hei⟩ := Indep.exists_insert_of_not_base (by simpa) h₁ h₂
+    have heI : e ∉ I := fun heI ↦ he' (mem_image_of_mem f heI)
+    rw [← image_insert_eq, restrict_indep_iff] at hei
+    exact ⟨e, ⟨he, heI⟩, hei.1, (injOn_insert heI).2 ⟨hIinj, he'⟩⟩ )
   ( by
-    rintro X hXE I ⟨hI, hIinj, hIE⟩ hIX
-    set M' := M ↾ (f '' E)
-    have hI' : M'.Indep (f '' I) := restrict_indep_iff.2 ⟨hI, image_subset f hIE⟩ 
-    obtain ⟨J, hJX, hIJ⟩ := hI'.subset_basis_of_subset (image_subset f hIX) (image_subset f hXE)
-    obtain ⟨J, hIJ', hJX', hJinj, rfl⟩ := hIinj.exists_injOn_superset_image hIX hIJ hJX.subset    
-    refine ⟨J, ⟨⟨hJX.indep.of_restrict, hJinj, hJX'.trans hXE⟩, hIJ', hJX'⟩, ?_⟩ 
-    rintro B ⟨⟨hB, hBinj, hBE⟩, -, hBX⟩ (hJB : J ⊆ B) b hb
-    have hB' : M'.Indep (f '' B) := restrict_indep_iff.2 ⟨hB, image_subset f hBE⟩ 
-    have hb' := mem_image_of_mem f hb
-    rw [←hJX.eq_of_subset_indep hB' (image_subset f hJB) (image_subset f hBX)] at hb'
-    exact hBinj.mem_of_mem_image hJB hb hb' )
-  ( fun I h ↦ h.2.2 )
+    rintro X - I ⟨hI, hIinj⟩ hIX
+    obtain ⟨J, hJ⟩ := (M ↾ range f).existsMaximalSubsetProperty_indep (f '' X) (by simp)
+      (f '' I) (by simpa) (image_subset _ hIX)
+    simp only [restrict_indep_iff, image_subset_iff, mem_maximals_iff, mem_setOf_eq, and_imp] at hJ
 
-@[simp] theorem preimage_indep_iff {M : Matroid β} : 
-    (M.preimage E f).Indep I ↔ (M.Indep (f '' I) ∧ InjOn f I ∧ I ⊆ E) := by 
+    obtain ⟨J₀, hIJ₀, hJ₀X, hbj⟩ := hIinj.bijOn_image.extend_of_subset hIX
+      (image_subset f hJ.1.2.1) (image_subset_iff.2 <| preimage_mono hJ.1.2.2)
+
+    have him := hbj.image_eq; rw [image_preimage_eq_of_subset hJ.1.1.2] at him; subst him
+    use J₀
+    simp only [mem_maximals_iff, mem_setOf_eq, hJ.1.1.1, hbj.injOn, and_self, hIJ₀,
+      hJ₀X, and_imp, true_and]
+    intro K hK hinj hIK hKX hJ₀K
+    rw [←hinj.image_eq_image_iff_of_subset hJ₀K Subset.rfl,
+       hJ.2 hK (image_subset_range _ _) ?_ (image_subset _ hKX) (image_subset _ hJ₀K)]
+    exact fun e he ↦ ⟨e, hIK he, rfl⟩ )
+  ( fun I hI e heI ↦ hI.1.subset_ground ⟨e, heI, rfl⟩ )
+
+@[simp] theorem preimage_indep_iff {M : Matroid β} :
+    (M.preimage f).Indep I ↔ M.Indep (f '' I) ∧ InjOn f I := by
   simp [preimage]
 
-@[simp] theorem preimage_ground_eq {M : Matroid β} : 
-    (M.preimage E f).E = E := rfl 
+@[simp] theorem preimage_ground_eq {M : Matroid β} :
+    (M.preimage f).E = f ⁻¹' M.E := rfl
+
+/-- The pullback of a matroid on `β` by a function `f : α → β` to a matroid on `α`, restricted
+  to a ground set `E`. Elements with the same image are parallel. -/
+def preimage' (M : Matroid β) (E : Set α) (f : α → β) : Matroid α := (M.preimage f) ↾ E
+
+@[simp] theorem preimage'_indep_iff {M : Matroid β} :
+    (M.preimage' E f).Indep I ↔ (M.Indep (f '' I) ∧ InjOn f I ∧ I ⊆ E) := by
+  simp [preimage', and_assoc]
+
+@[simp] theorem preimage'_ground_eq {M : Matroid β} :
+    (M.preimage' E f).E = E := rfl
 
 /-- If `f` is locally a bijection, then `M` is isomorphic to its preimage. -/
-noncomputable def iso_preimage [_root_.Nonempty α] (M : Matroid β) {f : α → β} {E : Set α} 
-    (hf : BijOn f E M.E) : Iso (M.preimage E f) M := 
-  Iso.of_forall_indep 
+noncomputable def iso_preimage [_root_.Nonempty α] (M : Matroid β) {f : α → β} {E : Set α}
+    (hf : BijOn f E M.E) : Iso (M.preimage' E f) M :=
+  Iso.of_forall_indep
   hf.toLocalEquiv
-  ( by rw [BijOn.toLocalEquiv_source, preimage_ground_eq] )
+  ( by rw [BijOn.toLocalEquiv_source, preimage'_ground_eq] )
   hf.toLocalEquiv_target
-  ( by 
-    simp only [preimage_ground_eq, preimage_indep_iff, BijOn.toLocalEquiv_apply,
+  ( by
+    simp only [preimage'_ground_eq, preimage'_indep_iff, BijOn.toLocalEquiv_apply,
       and_iff_left_iff_imp]
     exact fun I hIE _ ↦ ⟨hf.injOn.mono hIE, hIE⟩ )
 
-section Image 
+section Image
 
 /-- Map a matroid `M` on `α` to a copy in `β` using a function `f` that is injective on `M.E` -/
 def image (M : Matroid α) (f : α → β) (hf : InjOn f M.E) : Matroid β := matroid_of_indep
   ( f '' M.E )
-  ( fun I ↦ ∃ I₀, M.Indep I₀ ∧ I = f '' I₀) 
+  ( fun I ↦ ∃ I₀, M.Indep I₀ ∧ I = f '' I₀)
   ⟨ ∅, by simp ⟩
   ( by
-    rintro I _ ⟨J, hJ, rfl⟩ hIJ 
-    refine ⟨f ⁻¹' I ∩ M.E, hJ.subset ?_, ?_⟩ 
-    · refine (inter_subset_inter_left M.E (preimage_mono hIJ)).trans ?_ 
+    rintro I _ ⟨J, hJ, rfl⟩ hIJ
+    refine ⟨f ⁻¹' I ∩ M.E, hJ.subset ?_, ?_⟩
+    · refine (inter_subset_inter_left M.E (preimage_mono hIJ)).trans ?_
       rw [hf.preimage_image_inter hJ.subset_ground]
     simp only [subset_antisymm_iff, image_subset_iff, inter_subset_left, and_true]
     rintro x hx
     obtain ⟨y, hy, rfl⟩ := hIJ hx
     exact ⟨_, ⟨hx, hJ.subset_ground hy⟩, rfl⟩ )
-  ( by 
+  ( by
     rintro _ B ⟨I, hI, rfl⟩ hImax hBmax
     simp only [mem_maximals_iff, mem_setOf_eq, forall_exists_index, and_imp, image_subset_iff,
-      not_and, not_forall, exists_prop, exists_and_left] at hBmax hImax 
-    obtain ⟨⟨B, hB, rfl⟩, hmax⟩ := hBmax 
-    obtain ⟨_, I', hI', rfl, hII', hne⟩ := hImax _ hI rfl 
+      not_and, not_forall, exists_prop, exists_and_left] at hBmax hImax
+    obtain ⟨⟨B, hB, rfl⟩, hmax⟩ := hBmax
+    obtain ⟨_, I', hI', rfl, hII', hne⟩ := hImax _ hI rfl
 
     have hIb : ¬ M.Base I
     · refine fun hIb ↦ hne ?_
-      rw [hIb.eq_of_subset_indep ?_ (subset_inter hII' hI.subset_ground), 
+      rw [hIb.eq_of_subset_indep ?_ (subset_inter hII' hI.subset_ground),
         hf.preimage_image_inter hI'.subset_ground]
       rwa [hf.preimage_image_inter hI'.subset_ground]
-    
+
     have hB : M.Base B
     · refine hB.base_of_maximal (fun J hJ hBJ ↦ ?_)
       have h_image := hmax  _ hJ rfl (image_subset _ hBJ)
       rwa [hf.image_eq_image_iff_of_subset hB.subset_ground hJ.subset_ground] at h_image
-      
+
     obtain ⟨e, he, hi⟩ := hI.exists_insert_of_not_base hIb hB
-    refine ⟨f e, ⟨mem_image_of_mem f he.1, fun h ↦ he.2 ?_⟩, ⟨_, hi, by rw [image_insert_eq]⟩⟩ 
+    refine ⟨f e, ⟨mem_image_of_mem f he.1, fun h ↦ he.2 ?_⟩, ⟨_, hi, by rw [image_insert_eq]⟩⟩
     rwa [hf.mem_image_iff hI.subset_ground (hB.subset_ground he.1)] at h )
-  ( by 
-    rintro X hX I ⟨I, hI, rfl⟩ hIX 
-    obtain ⟨X, hXE, rfl⟩ := exists_eq_image_subset_of_subset_image hX 
-    rw [hf.image_subset_image_iff_of_subset hI.subset_ground hXE] at hIX 
-    
-    obtain ⟨B, hB, hIB⟩ := hI.subset_basis_of_subset hIX 
-    refine ⟨f '' B, ?_⟩ 
+  ( by
+    rintro X hX I ⟨I, hI, rfl⟩ hIX
+    obtain ⟨X, hXE, rfl⟩ := exists_eq_image_subset_of_subset_image hX
+    rw [hf.image_subset_image_iff_of_subset hI.subset_ground hXE] at hIX
+
+    obtain ⟨B, hB, hIB⟩ := hI.subset_basis_of_subset hIX
+    refine ⟨f '' B, ?_⟩
     simp only [image_subset_iff, mem_maximals_iff, mem_setOf_eq, and_imp, forall_exists_index]
-    refine ⟨⟨⟨B, hB.indep, rfl⟩, hIB.trans <| subset_preimage_image _ _, 
-      hB.subset.trans <| subset_preimage_image _ _⟩, ?_⟩ 
+    refine ⟨⟨⟨B, hB.indep, rfl⟩, hIB.trans <| subset_preimage_image _ _,
+      hB.subset.trans <| subset_preimage_image _ _⟩, ?_⟩
     rintro _ K hK rfl - hKX hBK
-    
+
     rw [hB.eq_of_subset_indep hK]
     · have hss := subset_inter hBK hB.left_subset_ground
       rwa [hf.preimage_image_inter hK.subset_ground] at hss
     rwa [hf.image_subset_image_iff_of_subset hK.subset_ground hXE] at hKX )
   ( by rintro _ ⟨I, hI, rfl⟩; exact image_subset _ hI.subset_ground )
 
-@[simp] theorem image_ground (M : Matroid α) (f : α → β) (hf : InjOn f M.E) : 
-    (M.image f hf).E = f '' M.E := rfl 
+@[simp] theorem image_ground (M : Matroid α) (f : α → β) (hf : InjOn f M.E) :
+    (M.image f hf).E = f '' M.E := rfl
 
-@[simp] theorem image_indep_iff (M : Matroid α) (f : α → β) (hf : InjOn f M.E) (I : Set β) : 
-    (M.image f hf).Indep I ↔ ∃ I₀, M.Indep I₀ ∧ I = f '' I₀ := 
-  by simp [image] 
+@[simp] theorem image_indep_iff (M : Matroid α) (f : α → β) (hf : InjOn f M.E) (I : Set β) :
+    (M.image f hf).Indep I ↔ ∃ I₀, M.Indep I₀ ∧ I = f '' I₀ :=
+  by simp [image]
 
 /-- `M` is isomorphic to its image -/
 noncomputable def iso_image [_root_.Nonempty α] (M : Matroid α) (f : α → β) (hf : InjOn f M.E) :
     Iso M (M.image f hf)  :=
-  Iso.of_forall_indep hf.toLocalEquiv ( by simp ) ( by simp )  
-  ( by 
+  Iso.of_forall_indep hf.toLocalEquiv ( by simp ) ( by simp )
+  ( by
     simp only [InjOn.toLocalEquiv, BijOn.toLocalEquiv_apply, image_indep_iff]
-    refine fun I hIE ↦ ⟨fun hI ↦ ⟨I, hI, rfl⟩, fun ⟨I₀, hI₀, (h_eq : f '' _ = _)⟩ ↦ ?_⟩ 
+    refine fun I hIE ↦ ⟨fun hI ↦ ⟨I, hI, rfl⟩, fun ⟨I₀, hI₀, (h_eq : f '' _ = _)⟩ ↦ ?_⟩
     rw [hf.image_eq_image_iff_of_subset hIE hI₀.subset_ground] at h_eq
-    rwa [h_eq] )    
-  
+    rwa [h_eq] )
+
 
 end Image
-  
-
